# baseURI: http://promsns.org/def/lic
# imports: http://promsns.org/def/agr
# imports: http://schema.theodi.org/odrs/index.ttl
# imports: http://www.w3.org/ns/prov-o

@prefix : <http://promsns.org/def/lic#> .
@prefix agr: <http://promsns.org/def/agr#> .
@prefix dc: <http://purl.org/dc/elements/1.1/> .
@prefix dcterms: <http://purl.org/dc/terms/> .
@prefix owl: <http://www.w3.org/2002/07/owl#> .
@prefix prov: <http://www.w3.org/ns/prov#> .
@prefix rdf: <http://www.w3.org/1999/02/22-rdf-syntax-ns#> .
@prefix rdfs: <http://www.w3.org/2000/01/rdf-schema#> .
@prefix skos: <http://www.w3.org/2004/02/skos/core#> .
@prefix xsd: <http://www.w3.org/2001/XMLSchema#> .

agr:Requirement
  rdfs:subClassOf [
      rdf:type owl:Restriction ;
      owl:cardinality "1"^^xsd:nonNegativeInteger ;
      owl:onProperty skos:definition ;
    ] ;
.
<http://promsns.org/def/lic>
  rdf:type owl:Ontology ;
  dc:creator "Nicholas Car" ;
  dcterms:created "2016-09-18"^^xsd:date ;
  dcterms:creator <http://promsns.org/id/person/nicholascar> ;
  dcterms:modified "2016-10-13"^^xsd:date ;
  rdfs:comment """This ontology specialises the Agreements Ontology (http://promsnns.org/def/agr) to specifically address the needs of data licensing. It borrows heavily from the Creative Commons Rights Expression Language (http://labs.creativecommons.org/demos/ns/) and the Open Data Initiative's Open Data Rights Statement Vocabulary (http://schema.theodi.org/odrs/) but hopes to be far more useful for machine-reading applications such as smart repositories that can autonomously calculate when and how to provide access to datasets based on licensing conditions.

This ontology follows the pattern set in the Agreements ontology by defining a license as a collection of requirements for action ob behalf of parties wishing to access or use data. A requirement could be to reference the creator of the dataset in derived data (attribution) or not to use data for commercial purposes. This promotion of individual 'requirements' to first-class objects allows very many licenses to be assembled from a small set of requirements which alows reasonably easy to use and yet somewhat customisable licenses to be created which may be better or more practical than either just restricting data access or mandating the use of standard licenses such as Creative Commons Attribution 4.0; two extreem positions."""@en ;
  rdfs:label "Licenses ontology"@en ;
  owl:imports <http://promsns.org/def/agr> ;
  owl:imports <http://schema.theodi.org/odrs/index.ttl> ;
  owl:imports <http://www.w3.org/ns/prov-o> ;
  owl:versionInfo "v1.0" ;
.
:Adapt
  rdf:type agr:Requirement ;
  agr:requirementLevel agr:MAY ;
  dc:source "Creative commons CC-BY 4.0 text (https://creativecommons.org/licenses/by/4.0/)" ;
  skos:definition "Remix, transform, and build upon the material for any purpose, even commercially"@en ;
.
:Attribution
  rdf:type agr:Requirement ;
  agr:requirementLevel agr:MUST ;
  dc:source "Creative commons CC-BY 4.0 text (https://creativecommons.org/licenses/by/4.0/)" ;
  skos:definition "You must give appropriate credit, provide a link to the license, and indicate if changes were made. You may do so in any reasonable manner, but not in any way that suggests the licensor endorses you or your use."@en ;
.
<http://promsns.org/def/lic#CC-BY-4.0>
  rdf:type :License ;
.
:GA_Internal_use_only
  rdf:type agr:Requirement ;
  agr:requirementLevel agr:MUST ;
  rdfs:comment "Any user of this data must be an Agent within the org:Organisation Geoscience Australia"@en ;
  skos:definition "Data is for GA's internal use only"@en ;
.
:License
  rdf:type owl:Class ;
  rdfs:comment """This license class represents a license object such as that which is applied to intellectual works and specifies the conditions of their use. It is identical in concept to the License class presented by the Creative Commons Rights Expression Language class and the Open Data Rights Statement Vocabulary's License class that is derived from the CC class but it is different in construction. This license class is a entirely a collection of individual  requirements (agr:Requirements) and contains no instruction itself. For this reason it is modelled as a skos:Collection, not a skos:Concept.

Note that this License class is a trivial subclass of the Agreements ontology's Agreement class. The only things changed for this subclass are the names of the class and this descriptive text as an Agreement class object is also a skos:Collection of Requirements. This means a license is really just an agreement with a particular set of Requirements and applicable to a particular set of Agents (perhaps the generators and future users of data) and that there is nothing inherently different about a license or nothing about an Agreement which is not applicable to a License.

The American spelling is used where license with an 's' is the same for both license noun and verb as opposed to the Australian spelling which uses a 'c' for the noun."""@en ;
  rdfs:label "license"@en ;
  rdfs:subClassOf agr:Agreement ;
  skos:altLabel "licence"@en ;
.
:No_Additional_Restrictions
  rdf:type agr:Requirement ;
  agr:requirementLevel agr:MUST_NOT ;
  dc:source "Creative commons CC-BY 4.0 text (https://creativecommons.org/licenses/by/4.0/)" ;
  skos:definition "You may not apply legal terms or technological measures that legally restrict others from doing anything the license permits."@en ;
.
:No_Warranties_are_given
  rdf:type agr:Requirement ;
  agr:requirementLevel agr:MUST_NOT ;
  dc:source "Creative commons CC-BY 4.0 text (https://creativecommons.org/licenses/by/4.0/)" ;
  rdfs:comment "You may not require a warranty from the license issuer."@en ;
  skos:definition "No warranties are given. The license may not give you all of the permissions necessary for your intended use. For example, other rights such as publicity, privacy, or moral rights may limit how you use the material."@en ;
.
:Not_for_Public_Domain_work
  rdf:type agr:Requirement ;
  agr:requirementLevel agr:OPTIONAL ;
  dc:source "Creative commons CC-BY 4.0 text (https://creativecommons.org/licenses/by/4.0/)" ;
  skos:definition "You do not have to comply with the license for elements of the material in the public domain or where your use is permitted by an applicable exception or limitation."@en ;
.
:Passed_with_new_agreement
  rdf:type agr:Requirement ;
  agr:requirementLevel agr:MUST_NOT ;
  rdfs:comment "The Agreement which this Requirement pertains to does not allow Persons other than members of Geoscience Australia use this data."@en ;
  skos:definition "Data cannot be passed to the third party unless there is a new agreement between GA and RSES"@en ;
.
:RSES_ANU_GA
  rdf:type :License ;
  agr:requires :GA_Internal_use_only ;
  agr:requires :Passed_with_new_agreement ;
.
:Share
  rdf:type agr:Requirement ;
  agr:requirementLevel agr:MAY ;
  dc:source "Creative commons CC-BY 4.0 (https://creativecommons.org/licenses/by/4.0/)" ;
  skos:definition "Copy and redistribute the material in any medium or format"@en ;
.
:licenseIssuer
  rdf:type owl:ObjectProperty ;
  rdfs:comment "This property indicates who the issuer of a particular license instance is. It allows direct indication wich may be needed whe there are multiple Agents associated with an Entity and it is unclear who the issuer is."@en ;
  rdfs:domain :License ;
  rdfs:range prov:Agent ;
.
